Add equivalence relation plus some lemmas

src/QuerySemantic.v
@@ -26,10 +26,9 @@ Require Import Ssromega.
 
 Require Import SeqExtra.
 
-Require Import ValidFragments.
-Require Import QueryRewrite.
 
 Require Import NRGTNF.
+Require Import QueryRewrite.
 
 
 Section QuerySemantic.
@@ -46,193 +45,1766 @@ Section QuerySemantic.
   
   Implicit Type u : @node Name Vals.
   Implicit Type query : @Query Name Vals.
+  Implicit Type queries : seq (@Query Name Vals).
 
-  Transparent query_size.
+  Transparent qresponse_name.
 
-  Reserved Notation "⟦ φ 'in' u ⟧ˢ" (at level 40).
+  Lemma queries_size_0_nil (qs : seq (@Query Name Vals)) : queries_size qs == 0 -> qs = [::].
+  Proof.
+    by elim: qs => //=; case=> [f α | l f α | f α φ | l f α φ | t φ] qs IH /=; rewrite addn_eq0.
+  Qed.
+
+ 
+  Reserved Notation "⟦ φ ⟧ˢ 'in' u" (at level 40).
   
   Equations? execute_selection_set u (queries : seq (@Query Name Vals)) :
     seq (Name * ResponseNode) by wf (queries_size queries) :=
     {
-      execute_selection_set _ [::] := [::];
+      ⟦ [::] ⟧ˢ in _ := [::];
       
-      execute_selection_set u (InlineFragment t φ :: qs)
+      ⟦ InlineFragment t φ :: qs ⟧ˢ in u
         with does_fragment_type_apply s u.(type) t :=
         {
-        | true := execute_selection_set u (φ ++ qs);
-        | _ := execute_selection_set u qs
+        | true := ⟦ φ ++ qs ⟧ˢ in u;
+        | _ := ⟦ qs ⟧ˢ in u
         };
 
-      execute_selection_set u (SingleField f α :: qs)
-        with u.(fields) (Field f α) :=
-        {
-        | Some (inl value) => (f, Leaf (SingleValue value)) :: execute_selection_set u (filter_queries_with_label f qs);
-        | Some (inr values) => (f, Array (map (Leaf \o SingleValue) values)) :: execute_selection_set u (filter_queries_with_label f qs);
-        | None => (f, Leaf Null) :: execute_selection_set u (filter_queries_with_label f qs)
-        };
-      
-      execute_selection_set u (LabeledField l f α :: qs)
-        with u.(fields) (Field f α) :=
-        {
-        | Some (inl value) => (l, Leaf (SingleValue value)) :: execute_selection_set u (filter_queries_with_label l qs);
-        | Some (inr values) => (l, Array (map (Leaf \o SingleValue) values)) :: execute_selection_set u (filter_queries_with_label l qs);
-        | None => (l, Leaf Null) :: execute_selection_set u (filter_queries_with_label l qs)
-        };
-
-      
-      execute_selection_set u (NestedField f α φ :: qs)
+      ⟦ SingleField f α :: qs ⟧ˢ in u
         with lookup_field_in_type s u.(type) f :=
         {
-        | Some (Schema.Field _ _ (ListType ty)) => (f, Array [seq Object (execute_selection_set v (φ ++ merge_selection_sets (find_queries_with_label s v.(type) f qs))) | v <- neighbours_with_field g u (Field f α)]) :: execute_selection_set u (filter_queries_with_label f qs);
-        
-        | Some (Schema.Field _ _ (NT ty))
-            with ohead (neighbours_with_field g u (Field f α)) :=
+        | Some _
+            with u.(fields) (Field f α) :=
             {
-            | Some v => (f, Object (execute_selection_set v (φ ++ merge_selection_sets (find_queries_with_label s v.(type) f qs)))) :: execute_selection_set u (filter_queries_with_label f qs);
-            
-            | _ =>  (f, Leaf Null) :: execute_selection_set u (filter_queries_with_label f qs)
+            | Some (inl value) => (f, Leaf (SingleValue value)) :: ⟦ filter_queries_with_label f qs ⟧ˢ in u;
+            | Some (inr values) => (f, Array (map (Leaf \o SingleValue) values)) :: ⟦ filter_queries_with_label f qs ⟧ˢ in u;
+            | None => (f, Leaf Null) :: ⟦ filter_queries_with_label f qs ⟧ˢ in u  (* Should throw error? *)
             };
-
-        | None => (f, Leaf Null) :: execute_selection_set u (filter_queries_with_label f qs)
+        | _ := ⟦ qs ⟧ˢ in u (* Should throw error *)
         };
-
-       execute_selection_set u (NestedLabeledField l f α φ :: qs)
+      
+      ⟦ LabeledField l f α :: qs ⟧ˢ in u
         with lookup_field_in_type s u.(type) f :=
         {
-        | Some (Schema.Field _ _ (ListType ty)) => (l, Array [seq Object (execute_selection_set v (φ ++ merge_selection_sets (find_queries_with_label s v.(type) l qs))) | v <- neighbours_with_field g u (Field f α)]) :: execute_selection_set u (filter_queries_with_label l qs);
-        
-        | Some (Schema.Field _ _ (NT ty))
-            with ohead (neighbours_with_field g u (Field f α)) :=
+        | Some _
+            with u.(fields) (Field f α) :=
             {
-            | Some v => (l, Object (execute_selection_set v (φ ++ merge_selection_sets (find_queries_with_label s v.(type) l qs)))) :: execute_selection_set u (filter_queries_with_label l qs);
-            
-            | _ =>  (l, Leaf Null) :: execute_selection_set u (filter_queries_with_label l qs)
+            | Some (inl value) => (l, Leaf (SingleValue value)) :: ⟦ filter_queries_with_label l qs ⟧ˢ in u;
+            | Some (inr values) => (l, Array (map (Leaf \o SingleValue) values)) :: ⟦ filter_queries_with_label l qs ⟧ˢ in u;
+            | None => (l, Leaf Null) :: ⟦ filter_queries_with_label l qs ⟧ˢ in u (* Should throw error? *)
             };
 
-        | None => (l, Leaf Null) :: execute_selection_set u (filter_queries_with_label l qs)
+        | _ := ⟦ qs ⟧ˢ in u (* Should throw error *)
+        };
+
+      
+      ⟦ NestedField f α φ :: qs ⟧ˢ in u 
+        with lookup_field_in_type s u.(type) f :=
+        {
+        | Some fld
+            with fld.(return_type) :=
+            {
+            |  ListType _ := (f, Array [seq Object (⟦ φ ++ merge_selection_sets (find_queries_with_label s f u.(type) qs) ⟧ˢ in v) | v <- neighbours_with_field g u (Field f α)])
+                              :: ⟦ filter_queries_with_label f qs ⟧ˢ in u;
+            | NT _
+                with ohead (neighbours_with_field g u (Field f α)) :=
+                {
+                | Some v => (f, Object (⟦ φ ++ merge_selection_sets (find_queries_with_label s f u.(type) qs) ⟧ˢ in v)) :: ⟦ filter_queries_with_label f qs ⟧ˢ in u;
+                
+                | _ =>  (f, Leaf Null) :: ⟦ filter_queries_with_label f qs ⟧ˢ in u
+                }
+            };
+
+        | None => ⟦ qs ⟧ˢ in u (* Should throw error *)
+        };
+
+      execute_selection_set u (NestedLabeledField l f α φ :: qs)
+        with lookup_field_in_type s u.(type) f :=
+        {
+        | Some fld
+            with fld.(return_type) :=
+            {
+            |  ListType _ := (l, Array [seq Object (⟦ φ ++ merge_selection_sets (find_queries_with_label s l u.(type) qs) ⟧ˢ in v) | v <- neighbours_with_field g u (Field f α)])
+                              :: ⟦ filter_queries_with_label l qs ⟧ˢ in u;
+            | NT _
+                with ohead (neighbours_with_field g u (Field f α)) :=
+                {
+                | Some v => (l, Object (⟦ φ ++ merge_selection_sets (find_queries_with_label s l u.(type) qs) ⟧ˢ in v)) :: ⟦ filter_queries_with_label l qs ⟧ˢ in u;
+                
+                | _ =>  (l, Leaf Null) :: ⟦ filter_queries_with_label l qs ⟧ˢ in u
+                }
+            };
+
+        | None => ⟦ qs ⟧ˢ in u (* Should throw error *)
         }
 
     }
-  where "⟦ queries 'in' u ⟧ˢ" := (execute_selection_set u queries).
+  where "⟦ queries ⟧ˢ 'in' u" := (execute_selection_set u queries).
+  Proof.
+    all: do [simp query_size; do ? ssromega].
+    all: do ?[by have Hleq := (filter_queries_with_label_leq_size f qs); ssromega].
+    all: do ?[by have Hleq := (filter_queries_with_label_leq_size l qs); ssromega].
   
-  all: do ?[by have Hleq := (filter_queries_with_label_leq_size f qs); ssromega].
-  all: do ?[by have Hleq := (filter_queries_with_label_leq_size l qs); ssromega].
+    all: do ?[by rewrite queries_size_app;
+            have Hleq1 := (found_queries_leq_size s f u.(type) qs);
+            have Hleq2 := (merged_selections_leq (find_queries_with_label s f u.(type) qs)); ssromega].
 
-  all: do ?[by rewrite -/(queries_size φ) queries_size_app;
-            have Hleq1 := (found_queries_leq_size s v.(type) f qs);
-            have Hleq2 := (merged_selections_leq (find_queries_with_label s v.(type) f qs)); ssromega].
-
-  all: do ?[by rewrite -/(queries_size φ) queries_size_app;
-            have Hleq1 := (found_queries_leq_size s v.(type) l qs);
-            have Hleq2 := (merged_selections_leq (find_queries_with_label s v.(type) l qs)); ssromega].
+    all: do ?[by rewrite queries_size_app;
+            have Hleq1 := (found_queries_leq_size s l u.(type) qs);
+            have Hleq2 := (merged_selections_leq (find_queries_with_label s l u.(type) qs)); ssromega].
 
 
-  all: do ? [by rewrite -/(queries_size φ) ?queries_size_app; ssromega].
+    all: do ? [by rewrite ?queries_size_app; ssromega].
   Qed.
 
-  Equations has_response_name : Name -> @Query Name Vals -> bool :=
+   
+  Lemma filter_queries_with_label_cat l (qs1 qs2 : seq (@Query Name Vals)) :
+    filter_queries_with_label l (qs1 ++ qs2) = filter_queries_with_label l qs1 ++ filter_queries_with_label l qs2.
+  Proof.
+    elim: qs1  => //= hd tl IH.
+    case: hd => //=; intros; simp filter_queries_with_label; do ?[by case: eqP => //= Heq; rewrite IH].
+    by rewrite IH.
+  Qed.
+  
+  Lemma find_queries_with_label_cat l ty (qs1 qs2 : seq (@Query Name Vals)):
+    find_queries_with_label s l ty (qs1 ++ qs2) = find_queries_with_label s l ty qs1 ++ find_queries_with_label s l ty qs2.
+  Admitted.
+
+
+
+  
+
+  (* Equations? Equiv (ty : Name) (φ φ' : seq (@Query Name Vals)) : bool by wf (queries_size φ) := *)
+  (*   { *)
+  (*     Equiv ty [::] [::] := true; *)
+
+  (*     Equiv ty (SingleField f α :: φ) (SingleField f' α' :: φ') := *)
+  (*       [&& f == f', *)
+  (*        α == α' & *)
+  (*        Equiv ty (filter_queries_with_label f φ) (filter_queries_with_label f φ')]; *)
+
+  (*     Equiv ty (NestedField f α β :: φ) (NestedField f' α' χ :: φ') *)
+  (*       with f == f', α == α' := *)
+  (*       { *)
+  (*       | true | true *)
+  (*                  with lookup_field_in_type s ty f := *)
+  (*                  { *)
+  (*                  | Some fld := let collected := find_queries_with_label s f ty φ in *)
+  (*                               let collected' := find_queries_with_label s f ty φ' in *)
+  (*                               all_eq ty (β ++ merge_selection_sets collected) (χ ++ merge_selection_sets collected') && (Equiv ty (filter_queries_with_label f φ) (filter_queries_with_label f φ')); *)
+  (*                  | _ := Equiv ty φ φ' *)
+  (*                  }; *)
+  (*       | _ | _ := false *)
+  (*       }; *)
+
+  (*     Equiv _ _ _ := false *)
+  (*   } *)
+  (* where all_eq (ty : Name) (φ φ' : seq (@Query Name Vals)) : bool := *)
+  (*         { *)
+  (*           all_eq ty φ φ' := all (fun t => Equiv t φ φ') (get_possible_types s ty) *)
+  (*         }. *)
+  
+  (* where "ty '⊢' φ '~' φ'" := (Equiv ty φ φ'). *)
+  (* Proof. *)
+  (*   all: do [simp query_size]. *)
+  (*   have Hleq := (filter_queries_with_label_leq_size f φ); ssromega. *)
+  (*   rewrite queries_size_app. *)
+  (*   have Hleq1 := (found_queries_leq_size s f ty φ). *)
+  (*   have Hleq := (merged_selections_leq collected). *)
+  (*   rewrite /collected in Hleq *; ssromega. *)
+  (*   have Hleq := (filter_queries_with_label_leq_size f φ); ssromega. *)
+  (*   ssromega. *)
+  (* Qed. *)
+  
+  
+
+  (* Equations? Equiv (ty : Name) (φ φ' : seq (@Query Name Vals)) : bool by wf (queries_size φ) := *)
+  (*   { *)
+  (*     ty ⊢ [::] ≡ [::] := true; *)
+
+  (*     ty ⊢ SingleField f α :: φ ≡ SingleField f' α' :: φ' := [&& f == f', *)
+  (*                                                            α == α' & *)
+  (*                                                            ty ⊢ filter_queries_with_label f φ ≡ filter_queries_with_label f φ']; *)
+
+  (*     ty ⊢ NestedField f α β :: φ ≡ NestedField f' α' χ :: φ' *)
+  (*       with f == f', α == α' := *)
+  (*       { *)
+  (*       | true | true *)
+  (*           with lookup_field_in_type s ty f := *)
+  (*           { *)
+  (*           | Some fld := *)
+  (*                        all_eq (get_possible_types s ty) && *)
+  (*                               (ty ⊢ filter_queries_with_label f φ ≡ filter_queries_with_label f φ') *)
+  (*                        where all_eq (tys : seq Name) : bool := *)
+  (*                                { *)
+  (*                                  all_eq [::] := true; *)
+  (*                                  all_eq (t :: tys) := t ⊢ (β ++ merge_selection_sets (find_queries_with_label s f ty φ)) ≡ *)
+  (*                                                        (χ ++ merge_selection_sets (find_queries_with_label s f ty φ')) *)
+  (*                                }; *)
+  (*                  | _ := ty ⊢ φ ≡ φ' *)
+  (*                  }; *)
+  (*       | _ | _ := false *)
+  (*       }; *)
+
+  (*     ty ⊢ InlineFragment t β :: φ ≡ φ' *)
+  (*       with is_fragment_spread_possible s t ty := *)
+  (*       { *)
+  (*       | true :=  *)
+  (*     _ ⊢ _ ≡ _ := false *)
+  (*   } *)
+ 
+  (* where "ty '⊢' φ '≡' φ'" := (Equiv ty φ φ'). *)
+  (* Proof. *)
+  (*   all: do [simp query_size]. *)
+  (*   have Hleq := (filter_queries_with_label_leq_size f φ); ssromega. *)
+  (*   rewrite queries_size_app. *)
+  (*   have Hleq1 := (found_queries_leq_size s f ty φ). *)
+  (*   have Hleq := (merged_selections_leq (find_queries_with_label s f ty φ)); ssromega. *)
+  (*   have Hleq := (filter_queries_with_label_leq_size f φ); ssromega. *)
+  (*   ssromega. *)
+  (* Qed. *)
+
+
+  Lemma merge_selection_sets_cat (qs1 qs2 : seq (@Query Name Vals)) :
+    merge_selection_sets (qs1 ++ qs2) = merge_selection_sets qs1 ++ merge_selection_sets qs2.
+  Admitted.
+  
+  Reserved Notation "ty '⊢' φ '≡' φ'" (at level 80).
+
+  
+  Inductive Equiv (ty : Name) : seq Query -> seq (@Query Name Vals) -> Prop :=
+  | ENil : ty ⊢ [::] ≡ [::]
+              
+  | ESF : forall f α φ φ',
+      ty ⊢ filter_queries_with_label f φ ≡ filter_queries_with_label f φ'  ->
+      ty ⊢ SingleField f α :: φ ≡ SingleField f α :: φ' 
+         
+ 
+  | ENF1 : forall f α β χ fld φ φ',
+      lookup_field_in_type s ty f = Some fld ->
+      (forall t, t \in get_possible_types s fld.(return_type) ->
+                  t ⊢ β ++ merge_selection_sets (find_queries_with_label s f ty φ) ≡
+                    χ ++ merge_selection_sets (find_queries_with_label s f ty φ')) ->
+      
+      ty ⊢ filter_queries_with_label f φ ≡ filter_queries_with_label f φ' ->
+      ty ⊢ NestedField f α β :: φ ≡ NestedField f α χ :: φ' 
+
+  | ENF2 : forall f α β χ φ φ',
+      lookup_field_in_type s ty f = None ->
+      ty ⊢ φ ≡ φ'  ->
+      ty ⊢ NestedField f α β :: φ ≡ NestedField f α χ :: φ' 
+
+  | EIF11 : forall t β φ φ',
+      does_fragment_type_apply s t ty ->
+      ty ⊢ β ++ φ ≡ φ'  ->
+      ty ⊢ InlineFragment t β :: φ ≡ φ' 
+
+  | EIF12 : forall t β φ φ',
+      does_fragment_type_apply s t ty ->
+      ty ⊢ φ' ≡ β ++ φ  ->
+      ty ⊢ φ' ≡ InlineFragment t β :: φ 
+         
+  | EIF21 : forall t β φ φ',
+      does_fragment_type_apply s t ty = false ->
+      ty ⊢ φ ≡ φ'  ->
+      ty ⊢ InlineFragment t β :: φ ≡ φ' 
+
+  | EIF22 : forall t β φ φ',
+      does_fragment_type_apply s t ty = false ->
+      ty ⊢ φ' ≡ φ  ->
+      ty ⊢ φ' ≡  InlineFragment t β :: φ 
+
+      
+  where "ty '⊢' φ '≡' φ' " := (Equiv ty φ φ').
+
+
+  Lemma equiv_sym ty φ φ' :
+    ty ⊢ φ ≡ φ' ->
+    ty ⊢ φ' ≡ φ.
+  Proof.
+    elim; intros.
+    - by constructor.
+    - by constructor.
+    - apply: ENF1 => //=.
+      * exact: H.
+      * by apply: H1.
+
+    - by apply: ENF2 => //=.
+
+    - by apply: EIF12 => //=.
+    - by apply: EIF11 => //=.
+    - by apply: EIF22 => //=.
+      by apply: EIF21 => //=.
+  Qed.
+
+  Hint Constructors Equiv.
+  Hint Resolve queries_size_app.
+  Lemma equiv_refl ty φ : ty ⊢ φ ≡ φ.
+  Proof.
+    move: {2}(queries_size _) (leqnn (queries_size φ)) => n.
+    elim: n ty φ => //= [| n IH] ty φ; first by rewrite leqn0 => /queries_size_0_nil ->; constructor.
+    case: φ; first by intros; constructor.
+    case=> //= [f α | | f α β | | t β] φ; simp query_size => Hleq.
+    - by constructor; apply: IH; have Hfleq := (filter_queries_with_label_leq_size f φ); ssromega.
+    - admit.
+    - case Hlook : (lookup_field_in_type s ty f) => [fld|] //=; [apply: ENF1 | apply: ENF2 => //].
+      * exact: Hlook.
+      * move=> t Hin.
+        apply: IH => /=.
+        rewrite queries_size_app.
+        admit.
+        admit.
+      * apply: IH; ssromega.
+
+    - admit.
+    - case Hspread : (does_fragment_type_apply s t ty) => //=; [apply: EIF11 => //= | apply: EIF21 => //=].
+      * apply: equiv_sym.
+        apply: EIF11 => //=.
+        apply: IH => //=.
+        rewrite queries_size_app; ssromega.
+
+      * apply: equiv_sym.
+        apply: EIF21 => //=; apply: IH; ssromega.
+  Admitted.
+
+  Hint Resolve equiv_refl.
+    
+
+  Lemma equiv_trans ty φ1 φ2 φ3 :
+    ty ⊢ φ1 ≡ φ2 ->
+    ty ⊢ φ2 ≡ φ3 ->
+    ty ⊢ φ1 ≡ φ3.
+  Proof.
+  Admitted.
+
+  
+
+  Lemma equiv_cat_hd ty φ1 φ1' φ :
+    ty ⊢ φ1 ≡ φ1' ->
+    ty ⊢ φ1 ++ φ ≡ φ1' ++ φ.
+  Proof.
+    move=> Heq.
+    elim: Heq φ => //=.
+    - intros; constructor.
+      by rewrite !filter_queries_with_label_cat; apply: H0.
+
+    - intros; apply: ENF1 => //=.
+      exact: H.
+      intros.
+      rewrite !find_queries_with_label_cat !merge_selection_sets_cat !catA.
+      apply: H1 => //=.
+      rewrite !filter_queries_with_label_cat; apply: H3.
+
+    - by intros; apply: ENF2.
+      
+    - intros; apply: EIF11 => //=.
+      by rewrite catA; apply: H1.
+
+    - by intros; apply: EIF12 => //=; rewrite catA; apply: H1.
+
+    - by intros; apply: EIF21.
+
+    - by intros; apply: EIF22.
+  Qed.
+
+  Lemma filter_swap f1 f2 (φ : seq (@Query Name Vals)) :
+    filter_queries_with_label f1 (filter_queries_with_label f2 φ) =
+    filter_queries_with_label f2 (filter_queries_with_label f1 φ).
+  Admitted.
+
+   Lemma filter_ground_swap k ty qs :
+    filter_queries_with_label k (ground s ty qs) = ground s ty (filter_queries_with_label k qs).
+  Admitted.
+  
+  
+  Lemma filter_preserves_equiv ty f φ φ' :
+    ty ⊢ φ ≡ φ' ->
+    ty ⊢ filter_queries_with_label f φ ≡ filter_queries_with_label f φ'.
+  Proof.
+    move: {2}(queries_size _) (leqnn (queries_size φ)) => n.
+    elim: n ty φ φ' => //= [| n IH] ty φ φ'.
+    - rewrite leqn0 => /queries_size_0_nil ->.
+      admit.
+
+    - case: φ => //=.
+    - admit.
+    - case=> [f' α | | f' α β | | t β] φ; simp query_size => /= Hleq.
+
+    - move=> Heq; inversion Heq.
+      * simp filter_queries_with_label; case: eqP => //= Hfeq.
+        by rewrite -Hfeq.
+        constructor. rewrite filter_swap [X in _ ⊢ _ ≡ X]filter_swap.
+        apply: IH => //=.
+        admit.
+      * simp filter_queries_with_label; case: eqP => //= Hfeq.
+        apply: EIF12 => //=.
+        rewrite -filter_queries_with_label_cat; apply: IH => //=.
+        
+
+  Admitted.
+
+        
+  Lemma equiv_cat_tail ty φ1 φ2 φ :
+    ty ⊢ φ1 ≡ φ2 ->
+    ty ⊢ φ ++ φ1 ≡ φ ++ φ2.
+  Proof.
+    move: {2}(queries_size _) (leqnn (queries_size φ)) => n.
+    elim: n ty φ φ1 φ2 => //= [| n IH] ty φ φ1 φ2.
+    by rewrite leqn0 => /queries_size_0_nil ->; rewrite 2!cat0s.
+    case: φ => //=; case=> [f α | | f α β | | t β] φ; simp query_size => /= Hleq.
+
+    - intros; constructor.
+      by apply: filter_preserves_equiv; apply: IH.
+
+    - admit.
+
+    - intros; case Hlook : (lookup_field_in_type s ty f) => [fld|] /=.
+      * apply: ENF1 => //=; first exact: Hlook.
+        intros.
+        apply IH => //=; first by ssromega.
+        rewrite 2!find_queries_with_label_cat 2!merge_selection_sets_cat.
+        apply IH => //=.
+        admit. (* merge size ≤ n *)
+        admit. (* merge preserves equiv *)
+        
+        by apply: filter_preserves_equiv; apply: IH => //; ssromega.
+
+      * apply: ENF2 => //=; apply: IH => //=; ssromega.
+
+    - admit.
+
+    - intros; case Hfapplies : (does_fragment_type_apply s t ty).
+      * apply: EIF11 => //=.
+        apply: EIF12 => //=; rewrite 2!catA.
+        apply: IH => //=.
+        by rewrite queries_size_app; ssromega.
+
+      * apply: EIF21 => //=.
+        apply: EIF22 => //=.
+        by apply: IH => //=; ssromega.
+
+  Admitted.
+
+    
+  Theorem equiv_cat ty φ φ' β β' :
+    ty ⊢ φ ≡ φ' ->
+    ty ⊢ β ≡ β' ->
+    ty ⊢ φ ++ β ≡ φ' ++ β'.
+  Proof.
+    move=> Heq1 Heq2.
+    have Heq11 := (equiv_cat_hd ty φ φ' β Heq1).
+    have Heq22 := (equiv_cat_tail ty β β' φ' Heq2).
+    apply: equiv_trans.
+    exact: Heq11.
+    exact: Heq22.
+  Qed.
+      
+
+    
+        
+  Lemma ground_cat ty (φ1 φ2 : seq (@Query Name Vals)) :
+    ground s ty (φ1 ++ φ2) = ground s ty φ1 ++ ground s ty φ2.
+  Admitted.
+  
+  Lemma ground_equiv1 ty φ1 φ2 :
+    forall t, t \in get_possible_types s ty ->
+               t ⊢ φ1 ≡ φ2  ->
+               t ⊢ ground s ty φ1 ≡ φ2.
+  Proof.
+    move: {2}(queries_size _) (leqnn (queries_size φ1)) => n.
+    elim: n ty φ1 φ2 => //= [| n IH] ty φ1 φ2.
+    - rewrite leqn0 => /queries_size_0_nil -> t Hin; simp ground.
+
+    - move=> Hleq t Hin Heq.
+      move: Hleq; inversion Heq => //=; simp query_size => Hleq; simp ground.
+
+    - case Hscope : is_object_type => //=.
+      * constructor.
+        rewrite filter_ground_swap.
+        apply: IH => //=.
+        admit. (* Size ≤ n *)
+
+      * simp try_inline_query; case: eqP => //= Hpty.
+          by rewrite Hpty in_nil in Hin.
+          admit. (* Inlining *)
+
+    - case Hlook : lookup_field_in_type => [fld'|] /=.
+      case Hscope : is_object_type => /=.
+      apply: ENF1 => //=.
+      * exact: H.
+      * intros.
+        have Httyeq : t = ty.
+          by rewrite (get_possible_types_objectE Hscope) /= mem_seq1 in Hin; apply/eqP.
+        rewrite Httyeq in IH H H0 Hlook *.
+        have Htrans : t0 ⊢ ground s fld'.(return_type) β ++ merge_selection_sets (find_queries_with_label s f ty (ground s ty φ)) ≡
+                                                       β ++ merge_selection_sets (find_queries_with_label s f ty φ).
+        apply: equiv_cat.
+        apply: IH => //=; [by ssromega | by rewrite Hlook in H; case: H => ->].
+        admit.
+
+
+        apply: equiv_trans.
+        exact: Htrans.
+        apply: H0 => //=.
+        rewrite filter_ground_swap; apply: IH => //=.
+        admit. (* Size ≤ n *)
+
+      simp try_inline_query; case: eqP => //= Hpty.
+      admit. (* same as before *)
+
+      admit. (* Inlining *)
+
+    - apply: equiv_sym. (* lookup = null case *)
+      admit.
+
+    - case Hlook : lookup_field_in_type => [fld |] //=.
+      case Hscope : is_object_type => /=.
+      * have Httyeq : t = ty.
+          by rewrite (get_possible_types_objectE Hscope) /= mem_seq1 in Hin; apply/eqP.
+          by rewrite Httyeq Hlook in H.
+
+      * (* Contradiction : field is found in ty but not in implementation *)
+        admit.
+
+      * admit. (* lookup = null *)
+
+
+    - case Hscope : is_object_type => //=.
+      * have Httyeq : t = ty.
+          by rewrite (get_possible_types_objectE Hscope) /= mem_seq1 in Hin; apply/eqP.
+
+        have Httyeq2 : t0 = ty.
+          by rewrite /does_fragment_type_apply Httyeq Hscope in H; apply/eqP.
+        rewrite Httyeq Httyeq2 in H H0 Hin *.
+        rewrite H /=.
+        rewrite -ground_cat.
+        apply: IH => //=.
+        rewrite queries_size_app; ssromega.
+      * case Ht : is_object_type => /=.
+        case Hfapplies : does_fragment_type_apply => /=.
+        apply: EIF11 => //=.
+        have Hteq : t0 = t by admit. (* Both are the same object *)
+        rewrite Hteq.
+        apply: equiv_trans.
+        apply: equiv_cat.
+        apply: IH => //=; [by ssromega|].
+        admit. (* object is subtype of object *)
+        by apply: IH => //=; ssromega.
+        exact: H0.
+
+        admit. (* Contradiction : t0 = t, pero no es subtipo de ty *)
+
+
+      * admit.
+
+    - apply: EIF12 => //=.
+      apply: IH => //=.
+      admit. (* Fail : Probably need to do induction over the sum of both lists' sizes ? *)
+
+    - case Hscope: is_object_type => /=.
+      * have -> /= : does_fragment_type_apply s ty t0 = false.
+        admit.
+          by apply: IH => //=; ssromega.
+      * case Ht : is_object_type => /=.
+        case Hfapplies : does_fragment_type_apply => /=.
+        apply: EIF21 => //=.
+        apply: IH => //=; ssromega.
+        apply: IH => //=; ssromega.
+
+      * admit.
+        
+    - apply: EIF22 => //=.
+      apply: IH => //=.
+        
+      
+  Theorem ground_equiv ty φ :
+    forall t, t \in get_possible_types s ty ->
+               t ⊢ ground s ty φ ≡ φ.
+  Proof.
+      by intros; apply: ground_equiv1.
+  Qed.
+
+  Theorem equiv_eval ty u φ φ' :
+    ty ⊢ φ ~ φ'  ->
+                   ⟦ φ ⟧ˢ in u = ⟦ φ' ⟧ˢ in u.
+  Proof.
+    move: {2}(queries_size _) (leqnn (queries_size φ)) => n.
+    elim: n ty u φ φ' => //= [| n IH] ty u φ φ'.
+    - rewrite leqn0 => /queries_size_0_nil ->. admit.
+    - move=> Hleq Heq.
+      case: Heq Hleq => //=.
+
+    - move=> f α fld φ1 φ2 Hlook Hfeq; simp query_size => Hleq.
+      simp execute_selection_set; rewrite Hlook /=.
+      case (u.(fields) _) => /= [[v | vs] |]; congr cons;
+      apply: (IH ty) => //=;
+      have Hfleq := (filter_queries_with_label_leq_size f φ1); ssromega.
+ 
+    - move=> f α φ1 φ2 Hlook *; simp execute_selection_set; rewrite Hlook /=.
+      by apply: (IH ty) => //=.
+
+
+    - move=> f α β χ fld φ1 φ2 Hlook Hseq Hfeq; simp query_size => Hleq.
+      simp execute_selection_set; rewrite Hlook /=.
+      case fld.(return_type) => rty /=.
+      * case ohead => [v |] /=;
+        congr cons; last by apply: (IH ty) => //=; have Hfleq := (filter_queries_with_label_leq_size f φ1); ssromega.
+        congr pair; congr Object.
+        apply: (IH u.(type) v) => //=.
+        rewrite queries_size_app.
+         have Hleq1 := (found_queries_leq_size s f u.(type) φ1).
+         have Hleq2 := (merged_selections_leq (find_queries_with_label s f u.(type) φ1)); ssromega.
+
+         apply: (IH ty) => //=.
+           by have Hfleq := (filter_queries_with_label_leq_size f φ1); ssromega.
+
+      *  congr cons;  last by apply: (IH ty) => //=; have Hfleq := (filter_queries_with_label_leq_size f φ1); ssromega.
+         congr pair; congr Array; apply/eq_in_map=> v Hin.
+         congr Object; apply: (IH u.(type) v) => //=.
+          rewrite queries_size_app.
+         have Hleq1 := (found_queries_leq_size s f u.(type) φ1).
+         have Hleq2 := (merged_selections_leq (find_queries_with_label s f u.(type) φ1)); ssromega.
+
+      * move=> f α β χ φ1 φ2 Hlook Heq; simp query_size => Hleq; simp execute_selection_set; rewrite Hlook /=.
+        apply: (IH ty) => //=; ssromega.
+
+    - move=> t β φ1 φ2 Happl Heq; simp query_size => Hleq; simp execute_selection_set; rewrite Happl /=.
+      apply: (IH ty) => //=; rewrite queries_size_app; ssromega.
+
+    - move=> t β φ1 φ2 Hnappl Heq; simp query_size => Hleq; simp execute_selection_set; rewrite Hnappl /=.
+      apply: (IH ty) => //=; ssromega.
+  Admitted.
+
+  Lemma empty_frag_equiv_nil ty u t (φ : seq (@Query Name Vals)) :
+    ty ⊢ [:: InlineFragment t [::]] ~ [::] in u.
+  Proof.
+    case Hfappl: (does_fragment_type_apply s u.(type) t) => /=.
+    apply: EIF1 => //=; constructor.
+    apply: EIF2 => //=; constructor.
+  Qed.
+
+  Lemma empty_frags_equiv_nil ty u pty :
+    ty ⊢ [seq InlineFragment t [::] | t <- pty] ~ [::] in u.
+  Proof.
+    elim: pty => //= [| t pty IH]; first by constructor.
+    case Hfappl: (does_fragment_type_apply s u.(type) t) => /=.
+    apply: EIF1 => //=.
+    by apply: EIF2.
+  Qed.
+
+    
+  Lemma inlining_equiv ty u pty f α :
+    ty ⊢ [seq InlineFragment t [:: SingleField f α] | t <- pty]  ~ 
+       [:: SingleField f α] in u.
+  Proof.
+    elim: pty => //= [| t pty IH].
+    - admit.
+    - case Happl: (does_fragment_type_apply s u.(type) t).
+
+      * apply: EIF1 => //=.
+        case Hlook : (lookup_field_in_type s u.(type) f) => [fld |] /=.
+        apply: ESF1; first exact: Hlook.
+        have /(_ pty) -> : forall qs, filter_queries_with_label f [seq InlineFragment t0 [:: SingleField f α] | t0 <- qs] =
+               [seq InlineFragment t0 [::] | t0 <- qs].
+        elim=> //= q qs IHqs; simp filter_queries_with_label => /=; case: eqP => //= _; simp filter_queries_with_label.
+        by rewrite IHqs.
+
+        simp filter_queries_with_label; apply: empty_frags_equiv_nil.
+
+        apply: ESF2 => //=.
+        admit.
+
+      * apply: EIF2 => //=.
+  Admitted.
+        
+        
+                                  
+  Lemma grounding_is_equiv ty u φ :
+    ty ⊢ ground s ty φ ~ φ in u.
+  Proof.
+    move: {2}(queries_size _) (leqnn (queries_size φ)) => n.
+    elim: n ty u φ => //= [| n IH] ty u φ.
+    - rewrite leqn0 => /queries_size_0_nil ->; simp ground; constructor.
+    - case: φ => [| q qs]; first by intros; simp ground; constructor.
+      case: q => [f α | | f α φ | | t φ]; simp query_size.
+
+    - move=> Hleq; simp ground.
+      case Hscope : is_object_type => /=.
+      case Hlook : (lookup_field_in_type s u.(type) f) => [fld|] /=.
+      apply: (ESF1 ty u f α fld) => //=.
+      admit.
+      apply: ESF2 => //=.
+      by apply: IH.
+
+    - simp try_inline_query; case: eqP => //= Hpty.
+      admit.
+      admit.
+
+    - admit.
+
+    - move=> Hleq; simp ground; case Hlook : lookup_field_in_type => [fld |] /=.
+      case Hscope : is_object_type => /=.
+      case Hlook2 : (lookup_field_in_type s u.(type) f) => [ufld |] /=.
+      apply: ENF1; first exact Hlook2.
+      move=> v.
+      
+      
+      
+      
+      
+      
+  Lemma find_filtered_neq_eq ty f f' qs :
+    f' <> f ->
+    find_queries_with_label s f' ty (filter_queries_with_label f qs) =
+    find_queries_with_label s f' ty qs.
+  Proof.
+    funelim (filter_queries_with_label f qs) => //= Hneq; rewrite /find_queries_with_label; simp ble => //=.
+    - case does_fragment_type_apply => //=;
+      rewrite -?/(find_queries_with_label s f' ty _);
+                                        rewrite ?H // ?H0 //.
+  Admitted.
+
+  
+  Lemma equiv_filter ty f φ φ' :
+    ty ⊢ φ ~ φ' ->
+    ty ⊢ filter_queries_with_label f φ ~ filter_queries_with_label f φ'.
+  Proof.
+    elim=> //= [| f' α qs1 qs2 Heq Hfeq]; simp filter_queries_with_label => /=.
+    - constructor.
+    - by case: eqP => //= _; constructor.
+    - (* move=> ty' uty f' α β χ fdef qs1 qs2 Heq Hfeq Hlook Hsbeq Hfsbeq.
+      simp filter_queries_with_label => /=; case: eqP => //= Hneq.
+      eapply ENF => //=.
+      apply: Hlook.
+      rewrite !find_filtered_neq_eq //.
+
+    - move=> ty' f' α β χ qs1 qs2 Heq Hfeq Hlook.
+      simp filter_queries_with_label => /=; case: eqP => //= _.
+      by constructor.
+  Qed.*)
+  Admitted.
+
+ 
+  Lemma equiv_cat_hd ty qs1 qs2 qs :
+    ty ⊢ qs1 ~ qs2 ->
+    ty ⊢ qs1 ++ qs ~ qs2 ++ qs.
+  Proof.
+    move: {2}(queries_size _) (leqnn (queries_size qs1)) => n.
+    elim: n qs qs1 qs2 ty => //= [| n IH] qs qs1 qs2 ty.
+    admit.
+
+    case: qs1 => /= [| q qs1 ] Hleq Heq.
+    by inversion Heq; rewrite cat0s; apply: equiv_refl.
+
+    move: Hleq; inversion Heq; simp query_size => Hleq; rewrite cat_cons.
+    
+    - by constructor; apply: IH.
+    
+    - by constructor; apply: IH.
+      
+    - apply: ENF => //.
+      apply: IH => //=. admit. (* ssromega. *)
+      exact: H3.
+      rewrite 2!find_queries_with_label_cat 2!merge_selection_sets_cat.
+      rewrite 2!catA.
+      apply: IH => //.
+      rewrite queries_size_app.
+      have Hleq1 := (found_queries_leq_size s f ty qs1).
+      have Hleq2 := (merged_selections_leq (find_queries_with_label s f ty qs1)).
+      ssromega.
+
+    - constructor => //; apply: IH => //. admit.
+  Admitted.
+
+   Lemma equiv_cat_tail ty qs1 qs2 qs :
+    ty ⊢ qs1 ~ qs2 ->
+    ty ⊢ qs ++ qs1 ~ qs ++ qs2.
+  Proof.
+  Admitted.
+
+  Lemma equiv_cat ty qs1 qs1' qs2 qs2' :
+    ty ⊢ qs1 ~ qs1' ->
+    ty ⊢ qs2 ~ qs2' ->
+    ty ⊢ qs1 ++ qs2 ~ qs1' ++ qs2'.
+  Proof.
+  Admitted.
+
+
+  Lemma ground_preserves_equiv ty φ :
+    ty ⊢ ground s ty φ ~ φ.
+  Proof.
+    elim: φ => //= [| q φ IH]; simp ground; first by constructor.
+
+    case: q; intros; simp ground.
+
+    - case is_object_type => //=.
+      * by constructor.
+      * simp try_inline_query; case: eqP => //= Hpty; first by constructor.
+        rewrite -[SingleField _ _ :: φ]cat1s.
+        apply: equiv_cat => //.
+  Admitted.
+  
+    
+  Lemma equiv_ble ty u φ φ' :
+    ty ⊢ φ ~ φ' ->
+    ⟦ φ ⟧ˢ in u = ⟦ φ' ⟧ˢ in u.
+  Proof.
+    move: {2}(queries_size _) (leqnn (queries_size φ)) => n.
+    elim: n ty u φ φ' => //= [| n IH] ty u φ φ'.
+    - admit. 
+    - case: φ => //= [| q φ] Hleq Heq; first by inversion Heq.
+
+      case:  q Heq Hleq; intros.
+
+      * inversion Heq.
+        simp execute_selection_set; case Hlook : lookup_field_in_type => [fld|] //=.
+        case (u.(fields) _) => [[v | vs] |] /=; congr cons; apply: IH; do ? by apply: (equiv_filter ty).
+        admit.
+        admit.
+        admit.
+        apply: (IH ty) => //.
+
+      * admit.
+
+      * simp query_size in Hleq.
+        inversion Heq.
+        simp execute_selection_set => //=.
+        case Hlook: lookup_field_in_type => [fld|] /=; last apply: (IH ty) => //=.
+        case fld.(return_type) => rty /=.
+        case ohead => [v |] //=.
+        congr cons.
+        congr pair; congr Object.
+        apply: IH => //=.
+        admit.
+
+  Admitted.
+
+  Lemma ground_preserves_semantics ty u φ :
+    ⟦ ground s ty φ ⟧ˢ in u = ⟦ φ ⟧ˢ in u.
+  Proof.
+    apply: equiv_ble.
+    apply: ground_preserves_equiv.
+  Qed.
+
+        
+        
+
+  Inductive BaseRewrite (ty : NamedType) : seq Query -> seq (@Query Name Vals) -> Prop :=
+  | SF : forall f α qs,
+      BaseRewrite ty (SingleField f α :: qs ++ [:: SingleField f α]) (SingleField f α :: qs)
+
+  | NF : forall f α φ β qs,
+      find_queries_with_label s f ty qs = [::] ->
+      BaseRewrite ty (NestedField f α φ :: qs ++ [:: NestedField f α β]) (NestedField f α (φ ++ β) :: qs)
+
+
+  (* | IF_Spread : forall t φ1 φ,
+      BaseRewrite ty [:: InlineFragment t (φ1 :: φ)] [:: InlineFragment t [:: φ1]; InlineFragment t φ] *)
+
+  (* | IF_Wrap : forall qs,
+      BaseRewrite ty qs [:: InlineFragment ty qs] *)
+
+  | IF_Wrap : forall q1 qs,
+      BaseRewrite ty (q1 :: qs) (InlineFragment ty [:: q1] :: q1 :: qs) (* Unnecessary I think? *)
+                  
+  | IF_Absorb : forall t φ qs,
+      BaseRewrite ty (InlineFragment t [:: InlineFragment t φ] :: qs)
+                  (InlineFragment t φ :: qs)
+
+  | IF_Int : forall t to q1 qs,
+      to \in implementation s t ->
+             BaseRewrite ty (q1 :: qs) (InlineFragment to [:: q1] :: q1 :: qs)
+
+  | IF_Union : forall t to φ,
+      to \in union_members s t ->
+             BaseRewrite ty [:: InlineFragment t φ] [:: InlineFragment to φ]
+
+  | IF_Del : forall t1 t2 φ,
+      is_object_type s t1 ->
+      is_object_type s t2 ->
+      t1 <> t2 ->
+      BaseRewrite ty [:: InlineFragment t1 [:: InlineFragment t2 φ]] [::].
+
+
+  Lemma repeated_eval_same u q1 qs :
+    
+    ⟦ q1 :: q1 :: qs 
+  Lemma sf_preserves u qs1 qs2 :
+    BaseRewrite u.(type) qs1 qs2 ->
+    ⟦ qs1 ⟧ˢ in u = ⟦ qs2 ⟧ˢ in u.
+  Proof.
+    elim.
+    - move=> f α qs; simp execute_selection_set; case Hlook : lookup_field_in_type => [fld|] //=.
+      case (u.(fields) _) => [[v | vs] |] //=; congr cons.
+      all: do ? [by rewrite filter_queries_with_label_cat; simp filter_queries_with_label => /=; case: eqP => //= _;
+                                                                                                            simp filter_queries_with_label; rewrite cats0].
+      * admit. (* lookup = null *)
+
+    - move=> f α φ β qs Hfind; simp execute_selection_set; case Hlook : lookup_field_in_type => [fld|] //=.
+      case fld.(return_type) => rty /=.
+      * case ohead => [v |] /=; rewrite filter_queries_with_label_cat; simp filter_queries_with_label => /=.
+        rewrite find_queries_with_label_cat Hfind /=.
+        simp merge_selection_sets; rewrite cats0.
+        simp filter_queries_with_label.
+        rewrite /find_queries_with_label.
+        simp ble; case: eqP => //= _; simp ble; simp filter_queries_with_label.
+        by simp merge_selection_sets => /=; rewrite !cats0.
+
+        by case: eqP => //= _; simp filter_queries_with_label; rewrite cats0.
+
+      * congr cons.
+        congr pair; congr Array; apply/eq_in_map => v Hin.
+        rewrite find_queries_with_label_cat Hfind /=; simp merge_selection_sets; rewrite cats0.
+        rewrite /find_queries_with_label; simp ble; case: eqP => //= _.
+        by simp merge_selection_sets => /=; rewrite cats0.
+        rewrite filter_queries_with_label_cat; simp filter_queries_with_label => /=; case: eqP => //= _.
+        by simp filter_queries_with_label; rewrite cats0.
+         
+      * admit. (* lookup = null *)
+
+    - move=> φ1 φ; simp execute_selection_set; case Hfapplies : does_fragment_type_apply => /=.
+      rewrite cats0.
+      admit.
+        by simp execute_selection_set; rewrite Hfapplies /=.
+
+    - simp execute_selection_set; case Hfapplies : does_fragment_type_apply => //=.
+        by rewrite cats0.
+        admit. (* Contradiction - needs info on node *)
+
+    - simp execute_selection_set; case Hfapplies : does_fragment_type_apply => //=.
+      by simp execute_selection_set; rewrite Hfapplies.
+      
+  Admitted.
+  
+
+ Reserved Notation "⦃ queries 'in' u ⦄" (at level 50).
+  
+   Equations? execute_selection_set2 u (queries : seq (@Query Name Vals)) :
+    seq (Name * ResponseNode) by wf (queries_size queries) :=
     {
-      has_response_name l (InlineFragment _ φ) := has (has_response_name l) φ;
+      execute_selection_set2 _ [::] := [::];
 
-      has_response_name l q := (qresponse_name q _) == l
-    }.
+      execute_selection_set2 u (SingleField f α :: qs)
+        with lookup_field_in_type s u.(type) f :=
+        {
+        | Some _ 
+            with u.(fields) (Field f α) :=
+            {
+            | Some (inl value) => (f, Leaf (SingleValue value)) :: ⦃ qs in u ⦄;
+            | Some (inr values) => (f, Array (map (Leaf \o SingleValue) values)) :: ⦃ qs in u ⦄;
+            | None => (f, Leaf Null) :: ⦃ qs in u ⦄
+            };
+        | _ := ⦃ qs in u ⦄ (* Error *)
+        };
+      
+      execute_selection_set2 u (LabeledField l f α :: qs)
+        with lookup_field_in_type s u.(type) f :=
+        {
+        | Some _ 
+            with u.(fields) (Field f α) :=
+            {
+            | Some (inl value) => (l, Leaf (SingleValue value)) :: ⦃ qs in u ⦄;
+            | Some (inr values) => (l, Array (map (Leaf \o SingleValue) values)) :: ⦃ qs in u ⦄;
+            | None => (l, Leaf Null) : ⦃ qs in u ⦄
+            };
+        | _ := ⦃ qs in u ⦄ (* Error *)
+        };
 
-  Lemma filtered_queries_hasN_response_name l qs :
-    all (fun q => ~~has_response_name l q) (filter_queries_with_label l qs).
-  Proof.
-    funelim (filter_queries_with_label l qs) => //=; simp has_response_name => /=; do ? apply_andP.
-    by apply/hasPn/allP.
+      
+      execute_selection_set2 u (NestedField f α φ :: qs)
+        with lookup_field_in_type s u.(type) f :=
+        {
+        | Some fld
+            with fld.(return_type) :=
+            {
+            | ListType _ => (f, Array [seq Object (⦃ φ in v ⦄) | v <- neighbours_with_field g u (Field f α)]) :: ⦃ qs in u ⦄;
+        
+            | NT ty
+                with ohead (neighbours_with_field g u (Field f α)) :=
+                {
+                | Some v => (f, Object (⦃ φ in v ⦄)) :: ⦃ qs in u ⦄;
+                
+                | _ =>  (f, Leaf Null) :: ⦃ qs in u ⦄
+                }
+            };
+
+        | None => ⦃ qs in u ⦄ (* Error *)
+        };
+    execute_selection_set2 u (NestedLabeledField l f α φ :: qs)
+        with lookup_field_in_type s u.(type) f :=
+        {
+        | Some fld
+            with fld.(return_type) :=
+            {
+            | ListType _ => (l, Array [seq Object (⦃ φ in v ⦄) | v <- neighbours_with_field g u (Field f α)]) :: ⦃ qs in u ⦄;
+        
+            | NT ty
+                with ohead (neighbours_with_field g u (Field f α)) :=
+                {
+                | Some v => (l, Object (⦃ φ in v ⦄)) :: ⦃ qs in u ⦄;
+                
+                | _ =>  (l, Leaf Null) :: ⦃ qs in u ⦄
+                }
+            };
+
+        | None => ⦃ qs in u ⦄ (* Error *)
+        };
+
+       
+        execute_selection_set2 u (InlineFragment t φ :: qs)
+        with does_fragment_type_apply s u.(type) t :=
+        {
+        | true := ⦃ φ ++ qs in u ⦄;
+        | _ := ⦃ qs in u ⦄
+        }
+
+    }
+   where "⦃ queries 'in' u ⦄" := (execute_selection_set2 u queries).
+   all: do [simp query_size]; do ?by ssromega.
+     by rewrite queries_size_app; ssromega.
   Qed.
 
-  Lemma filter_queries_preserves_non_existent l qs l' :
-    all (fun q => ~~has_response_name l q) qs ->
-    all (fun q => ~~has_response_name l q) (filter_queries_with_label l' qs).
+
+
+   Lemma execute_selection_set2_cat u qs1 qs2 :
+    ⦃ qs1 ++ qs2 in u ⦄ = ⦃ qs1 in u ⦄ ++ ⦃ qs2 in u ⦄.
   Proof.
-    funelim (filter_queries_with_label l' qs) => //= /andP [Hp Hall]; simp has_response_name; apply_andP.
-    - apply/hasPn/allP. apply: H. simp has_response_name in Hp. move/hasPn/allP in Hp. done.
-    all: do ? by apply: H0.
-    all: do ? by apply: H.
+    move: {2}(queries_size _) (leqnn (queries_size qs1)) => n.
+    elim: n qs1 => // [| n IH] qs1.
+    - by rewrite leqn0 => /queries_size_0_nil ->. 
+    - case: qs1 => //=; case=> [f α | l f α | f α φ | l f α φ | t φ] qs; simp query_size => Hleq; simp execute_selection_set2.
+      * Admitted.
+
+  
+  Lemma all_invalid_fragments_eval u φ qs :
+    all (fun q => q.(is_inline_fragment)) qs ->
+    are_grounded s qs ->
+    all (fun q => ~~are_similar q (InlineFragment u.(type) φ)) qs ->
+    ⦃ qs in u ⦄ = [::].
+  Proof.
+    elim: qs => //=; case=> // t χ qs IH /andP [Hinl Hinls].
+    simp are_grounded; simp is_field.
+  Admitted.
+
+   Theorem execs_on_nrgtnf_are_equivalent u φ :
+    are_grounded s φ ->
+    are_non_redundant φ ->
+    ⦃ φ in u ⦄ = ⟦ φ ⟧ˢ in u.
+   Proof.
+   Admitted.
+   (*
+    move: {2}(queries_size _) (leqnn (queries_size φ)) => n.
+    elim: n φ u => [| n IH] φ u.
+    - by rewrite leqn0 => /queries_size_0_nil ->. 
+    - case: φ => //=; case=> /= [f α | l f α | f α φ | l f α φ | t φ] qs Hleq.
+      * simp are_grounded; simp is_field => /andP [Hflds Hnf].
+        simp are_non_redundant; rewrite andTb => /=-/andP [Hneq Hnr].
+        simp execute_selection_set; simp execute_selection_set2.
+        case: (u.(fields) _) => //=; [case=> // v|];
+                                 rewrite (filter_not_similar_preserves_list (SingleField f α)) // IH //; by apply: asdf.
+      
+      * simp are_in_normal_form => /andP [Hflds Hnf].
+        simp are_non_redundant; rewrite andTb => /=-/andP [Hneq Hnr].
+        simp execute_selection_set; simp execute_selection_set2.
+        case: (u.(fields) _) => //=; [case=> // v|];
+                                 rewrite (filter_not_similar_preserves_list (LabeledField l f α)) // IH //; by apply: asdf.
+
+        
+      * simp are_in_normal_form => /and3P [Hnf Hfields Hnfs].
+        simp are_non_redundant => /= /and3P [Hsim Hnr Hnrs]. 
+        simp execute_selection_set; simp execute_selection_set2.
+        case Hlook : lookup_field_in_type => [fld|] //=; last rewrite (filter_not_similar_preserves_list (NestedField f α φ)) //.
+        case: fld Hlook => f' args; case=> ty Hlook /=. 
+        + case ohead => //= [v|]; rewrite (filter_not_similar_preserves_list (NestedField f α φ)) //.
+          rewrite (find_not_similar_is_nil v.(type) (NestedField f α φ)) //; simp merge_selection_sets.
+          by rewrite cats0 !IH //; rewrite -/(queries_size φ) in Hleq; ssromega.
+          by rewrite IH //; ssromega.
+          
+        + rewrite (filter_not_similar_preserves_list (NestedField f α φ)) //. 
+          congr cons; last by apply: IH => //; ssromega.
+          congr pair; congr Array.
+          apply/eq_in_map => v Hin.
+          rewrite (find_not_similar_is_nil v.(type) (NestedField f α φ)) //; simp merge_selection_sets.
+            by rewrite cats0 !IH //; rewrite -/(queries_size φ) in Hleq; ssromega.
+        + by rewrite IH //; ssromega.
+             
+      * simp are_in_normal_form => /and3P [Hnf Hfields Hnfs].
+        simp are_non_redundant => /= /and3P [Hsim Hnr Hnrs]. 
+        simp execute_selection_set; simp execute_selection_set2.
+        case Hlook : lookup_field_in_type => [fld|] //=; last rewrite (filter_not_similar_preserves_list (NestedLabeledField l f α φ)) //.
+        case: fld Hlook => f' args; case=> ty Hlook /=. 
+        + case ohead => //= [v|]; rewrite (filter_not_similar_preserves_list (NestedLabeledField l f α φ)) //.
+          rewrite (find_not_similar_is_nil v.(type) (NestedLabeledField l f α φ)) //; simp merge_selection_sets.
+            by rewrite cats0 !IH //; rewrite -/(queries_size φ) in Hleq; ssromega.
+          by rewrite IH //; ssromega.
+         
+        + rewrite (filter_not_similar_preserves_list (NestedLabeledField l f α φ)) //. 
+          congr cons; last by apply: IH => //; ssromega.
+          congr pair; congr Array.
+          apply/eq_in_map => v Hin.
+          rewrite (find_not_similar_is_nil v.(type) (NestedLabeledField l f α φ)) //; simp merge_selection_sets.
+            by rewrite cats0 !IH //; rewrite -/(queries_size φ) in Hleq; ssromega.
+        + by rewrite IH //; ssromega.
+
+       
+      * simp are_in_normal_form => /and5P [Hobj Hflds Hnf Hinl Hnfs].
+        simp are_non_redundant => /= /and3P [Hsim Hnr Hnrs].
+        simp execute_selection_set; simp execute_selection_set2.
+        case Hfrag: does_fragment_type_apply => //=; last by apply: IH => //; ssromega.
+        rewrite execute_selection_set2_cat.
+        rewrite (all_invalid_fragments_eval u φ qs) // ?cats0; last first.
+        rewrite /does_fragment_type_apply Hobj in Hfrag.
+          by move/eqP in Hfrag; rewrite Hfrag.        
+        
+          
+        rewrite all_invalid_fragments_exec //; [apply: IH => //; rewrite -/(queries_size φ) in Hleq; ssromega|].
+        rewrite /does_fragment_type_apply Hobj in Hfrag.
+          by move/eqP in Hfrag; rewrite Hfrag.
+  Qed.
+
+    *)
+
+       
+  Lemma sf_evalE f α u qs :
+    [\/ exists value, ⟦ SingleField f α :: qs ⟧ˢ in u = (f, Leaf (SingleValue value)) :: ⟦ filter_queries_with_label f qs ⟧ˢ in u,
+       exists values, ⟦ SingleField f α :: qs ⟧ˢ in u = (f, Array (map (Leaf \o SingleValue) values)) :: ⟦ filter_queries_with_label f qs ⟧ˢ in u,
+       ⟦ SingleField f α :: qs ⟧ˢ in u = (f, Leaf Null) :: ⟦ filter_queries_with_label f qs ⟧ˢ in u |
+     ⟦ SingleField f α :: qs ⟧ˢ in u = ⟦ qs ⟧ˢ in u].
+  Proof.
+    simp execute_selection_set; case lookup_field_in_type => /= [fld|]; last by constructor 4.
+    by case (u.(fields) _) => [[v | vs]|]; [constructor 1; exists v | constructor 2; exists vs | constructor 3].
   Qed.
   
-  Transparent qresponse_name.
-  
-  Lemma exec_preserves_non_existent_label u qs l :
-    all (fun q => ~~has_response_name l q) qs ->
-    all (fun kq => kq.1 != l) (⟦ qs in u ⟧ˢ).
+ 
+  Lemma filter_remove_swap k (qs : seq (@Query Name Vals)) :
+    filter_queries_with_label k (remove_redundancies qs) = remove_redundancies (filter_queries_with_label k qs).
+  Admitted.
+
+  Lemma filter_filter_absorb k (qs : seq (@Query Name Vals)) :
+    filter_queries_with_label k (filter_queries_with_label k qs) = filter_queries_with_label k qs.
+  Admitted.
+
+   Lemma find_queries_or_fields_is_same_if_all_fields ty label qs :
+    all (fun q => q.(is_field)) qs ->
+    find_queries_with_label s label ty qs = find_fields_with_response_name Name Vals label qs.
   Proof.
-    funelim (execute_selection_set u qs) => //=; simp has_response_name => /= /andP [Hne Hall]; do ? apply_andP.
+    rewrite /find_queries_with_label.
+    elim: qs => //= q qs IH /andP [Hfield Hfields].
+    case: q Hfield => //= [f α | l f α | f α φ | l f α φ] _.
 
-    all: do ?[by apply: H; apply: filter_queries_preserves_non_existent].
-    all: do ?[by apply: H0; apply: filter_queries_preserves_non_existent].
-
-    by apply: H; rewrite all_cat; apply_andP; apply/allP/hasPn.
-    by apply: H.
+    all: do ?[by simp ble; simp find_fields_with_response_name;
+              case: eqP => //= _; [congr cons |]; apply: IH].
   Qed.
 
+  Lemma filtering_invalid_fragments_preserves_semantics t u qs :
+    are_grounded_inlines s qs -> 
+    does_fragment_type_apply s u.(type) t = false -> 
+    ⟦ filter_fragments_with_guard t qs ⟧ˢ in u = ⟦ qs ⟧ˢ in u.
+  Proof.
+    move: {2}(queries_size _) (leqnn (queries_size qs)) => n.
+    elim: n qs u t => /= [| n IH] qs u t.
+    - by rewrite leqn0 => /queries_size_0_nil ->. 
+    - case: qs => //=; case=> // t' φ qs; simp query_size => Hleq; simp is_grounded => /and3P [_ /andP [Htobj Hginls] Hgflds] Hfapplies.
+      simp filter_fragments_with_guard; case: eqP => //= [-> | Hneq]; simp execute_selection_set.
+      * by rewrite Hfapplies /=; apply: IH => //; ssromega.
+      * case: does_fragment_type_apply => //=; last by apply: IH => //; ssromega.
+        (* by apply: qwe; apply: IH => //; ssromega. *)
+  Admitted.
+
+                                 
+
+  Lemma eval_filter k qs1 qs2 u :
+    ⟦ qs1 ⟧ˢ in u = ⟦ qs2 ⟧ˢ in u ->
+    ⟦ filter_queries_with_label k qs1 ⟧ˢ in u = ⟦ filter_queries_with_label k qs2 ⟧ˢ in u.
+  Proof. 
+    move: {2}(queries_size _) (leqnn (queries_size qs1)) => n.
+    elim: n qs1 qs2 u => /= [| n IH] qs1 qs2 u.
+    - rewrite leqn0 =>  /queries_size_0_nil ->; simp execute_selection_set. admit.
+  Admitted.
   
+  Lemma eval1 qs qs1 qs2 u :
+    ⟦ qs1 ⟧ˢ in u = ⟦ qs2 ⟧ˢ in u ->
+    ⟦ qs ++ qs1 ⟧ˢ in u = ⟦ qs ++ qs2 ⟧ˢ in u.
+  Proof.
+    move: {2}(queries_size _) (leqnn (queries_size qs)) => n.
+    elim: n qs qs1 qs2 u => /= [| n IH] qs qs1 qs2 u.
+    - by rewrite leqn0 => /queries_size_0_nil ->. 
+    - case: qs => //; case=> [f α | l f α | f α φ | l f α φ | t φ] qs; simp query_size => Hleq Heq; rewrite 2!cat_cons.
+
+      * simp execute_selection_set; case lookup_field_in_type => [fld|] /=; last by apply: IH.
+        case (u.(fields) _) => [[v | vs] |] /=; congr cons; apply: eval_filter; apply: (IH qs qs1) => //=.
+                                (* filtering two equivalent queries preserves semantics *)
+        
+      * simp execute_selection_set; case lookup_field_in_type => [fld|] /=; last by apply: IH.
+        case (u.(fields) _) => [[v | vs] |] /=; congr cons;
+                                admit. (* filtering two equivalent queries preserves semantics *)
+        
+      * simp execute_selection_set; case lookup_field_in_type => [fld|] /=; last by apply: IH => //; ssromega.
+        case fld.(return_type) => /= rty.
+        + case ohead => [v |] /=.
+          congr cons.
+          congr pair; congr Object.
+          apply: (IH φ (merge_selection_sets (find_queries_with_label s f v.(type) (qs ++ qs1)))); first by ssromega.
+          admit. (* eval subqueries from similar fields is equiv *)
+          admit. (* filtering two equivalent queries preserves semantics *)
+          admit. (* filtering two equivalent queries preserves semantics *)
+
+        + congr cons.
+          congr pair; congr Array; apply/eq_in_map=> v Hin; congr Object.
+          apply: (IH φ (merge_selection_sets (find_queries_with_label s f v.(type) (qs ++ qs1)))); first by ssromega.
+          admit. (* eval subqueries from similar fields is equiv *)
+          admit. (* filtering two equivalent queries preserves semantics *)
+
+
+      * admit. (* Copy & Paste *) 
+       
+      * simp execute_selection_set; case does_fragment_type_apply => /=.
+        rewrite 2!catA; apply: IH => //; rewrite queries_size_app; ssromega.
+        by apply: IH => //; ssromega.
+  Admitted.
+  
+  
+  Theorem rem_red_ground_sem ty u qs :
+    are_grounded2 s ty qs ->
+    ⟦ remove_redundancies qs ⟧ˢ in u = ⟦ qs ⟧ˢ in u.
+  Proof.
+    move=> Hg.
+    rewrite -execs_on_nrgtnf_are_equivalent; [
+    | admit
+    | by apply: remove_redundancies_is_non_redundant].
+
+    funelim (remove_redundancies qs) => //=.
+    - simp execute_selection_set2; simp execute_selection_set.
+      case Hlook : lookup_field_in_type => [fld|] /=.
+      * case (u.(fields) _) => [[v | vs] |] /=; rewrite (H ty) //; admit. (* Filter preserves grounding *)
+      * admit. (* lookup = null *)
+
+    - admit. (* Copy & Paste *)
+
+    - simp execute_selection_set2; simp execute_selection_set.
+      case Hlook : lookup_field_in_type => [fld|] /=; last admit. (* lookup = null *)
+      case fld.(return_type) => rty /=.
+      * case ohead => [v |] /=.
+        rewrite (H rty) /=.
+        rewrite (H0 ty).
+        rewrite !find_queries_or_fields_is_same_if_all_fields //.
+        admit. (* all are fields *)
+        admit. (* Filter preserves grounding *)
+        admit. (* subqueries are grounded wtr field's type *)
+
+        rewrite (H0 ty) //; admit. (* Filter preserves grounding *)
+
+      * congr cons.
+        congr pair; congr Array; apply/eq_in_map=> v Hin; congr Object.
+        rewrite !find_queries_or_fields_is_same_if_all_fields.
+        rewrite (H rty) //.
+        admit. (* Subqueries are grounded *)
+        admit. (* All are fields *)
+        apply: (H0 ty); admit. (* Filter preserves grounding *)
+
+    - admit. (* Copy & Paste *)
+
+    - simp execute_selection_set2; simp execute_selection_set.
+      case Hfapplies : does_fragment_type_apply => //=.
+      rewrite execute_selection_set2_cat.
+      rewrite (H s6).
+      rewrite (H0 ty).
+  Admitted.
+      
+        
+
+  Lemma adfasqw f α ty qs u :
+    is_object_type s ty = false ->
+    get_possible_types s ty != [::] ->
+    ⦃ remove_redundancies ([seq InlineFragment ty0 [:: SingleField f α] | ty0 <- get_possible_types s ty] ++ ground s ty qs) in u ⦄ =
+    ⦃ [seq InlineFragment ty0 (SingleField f α :: merge_selection_sets (find_fragments_with_guard ty0 (ground s ty qs))) | ty0 <- get_possible_types s ty] in u⦄ .
+  Proof.
+    move=> Hscope Hptys.
+    
+    
+  Abort.
+    
+    
+   Theorem normalize_preserves_semantics ty u qs :
+     ⟦ normalize s ty qs ⟧ˢ in u = ⟦ qs ⟧ˢ in u.
+   Proof.
+     have [Hg Hnr] := (normalized_queries_are_in_normal_form Name Vals s ty qs).
+     rewrite -execs_on_nrgtnf_are_equivalent //.
+     rewrite /normalize /=.     
+     move: {2}(queries_size _) (leqnn (queries_size qs)) => n.
+     elim: n qs ty Hg Hnr u => [| n IH] qs ty Hg Hnr u.
+    - by rewrite leqn0 => /queries_size_0_nil ->. 
+    - case: qs Hg Hnr => //=; case=> [f α | l f α | f α φ | l f α φ | t φ] qs Hg Hnr; simp query_size => Hleq;
+      simp ground.
+     
+    - case Hscope : is_object_type => /=.
+      
+      simp remove_redundancies; simp execute_selection_set2; simp execute_selection_set.
+      case Hlook : lookup_field_in_type => [fld|] /=.
+      case (u.(fields) _) => [[v | vs] |] /=; rewrite filter_ground_swap IH //.
+      all: do ? by have [Hg' _] := (normalized_queries_are_in_normal_form Name Vals s ty (filter_queries_with_label f qs)).
+      all: do ? by have [_ Hnr'] := (normalized_queries_are_in_normal_form Name Vals s ty (filter_queries_with_label f qs)).
+      all: do ? by have Hfleq := (filter_queries_with_label_leq_size f qs); ssromega.
+      admit. (* lookup = ⊥ -> qs should evaluate to the same *)
+
+    - simp try_inline_query; case: eqP => //= Hpty.
+      * admit. (* Same as previous *)
+      * admit. (* Inlining field *)
+
+    - admit. (* Copy & Paste *)
+
+    - case Hlook1 : lookup_field_in_type => [fld |] /=.
+      case Hscope : is_object_type => /=.
+      simp remove_redundancies; simp execute_selection_set2.
+      simp execute_selection_set.
+      case Hlook2 : lookup_field_in_type => [fld2 |] /=.
+      case fld2.(return_type) => rty /=.
+      case ohead => [v |] /=; congr cons.
+      congr pair; congr Object.
+      admit.
+   Abort.
+     
+  
+
+
+        
+        
+
+  Lemma exec_filtered_queries_asdf u qs l :
+    all (fun kq => kq.1 != l) (⟦ filter_queries_with_label l qs ⟧ˢ in u).
+  Proof.
+    funelim (filter_queries_with_label l qs) => //=; simp execute_selection_set.
+    - 
+  Admitted.
+
+ 
   Lemma exec_responses_are_non_redundant u qs :
     Response.are_non_redundant (execute_selection_set u qs).
   Proof.
     apply_funelim (execute_selection_set u qs) => //=; clear u qs => u.
-    - move=> f α v qs IH Hv; simp is_non_redundant; rewrite andTb; apply_andP.
-      apply: exec_preserves_non_existent_label.
-      apply: filtered_queries_hasN_response_name.
-    - move=> f α vs qs IH Hv; simp is_non_redundant; apply_and3P.
-      * by rewrite all_map; apply/allP.
-      * apply: exec_preserves_non_existent_label.
-        apply: filtered_queries_hasN_response_name.
 
-    - move=> f α qs IH Hnull; simp is_non_redundant; rewrite andTb; apply_andP.
-      apply: exec_preserves_non_existent_label.
-      apply: filtered_queries_hasN_response_name.
-      
-    - move=> l f α v qs IH Hv; simp is_non_redundant; rewrite andTb; apply_andP.
-      apply: exec_preserves_non_existent_label.
-      apply: filtered_queries_hasN_response_name.
-    - move=> l f α vs qs IH Hv; simp is_non_redundant; apply_and3P.
-      * by rewrite all_map; apply/allP.
-      * apply: exec_preserves_non_existent_label.
-        apply: filtered_queries_hasN_response_name.
+    all: do ? by intros; apply_and3P; apply: exec_filtered_queries_asdf.
 
-    - move=> l f α qs IH Hnull; simp is_non_redundant; rewrite andTb; apply_andP.
-      apply: exec_preserves_non_existent_label.
-      apply: filtered_queries_hasN_response_name.
-
-    - move=> f f' args ftype α φ qs IH IHqs Hlook; simp is_non_redundant. apply_and3P.
-      * rewrite all_map; apply/allP => v Hin /=; simp is_non_redundant.
-      * apply: exec_preserves_non_existent_label.
-        apply: filtered_queries_hasN_response_name.
-
-    - move=> f α φ qs IH Hlook; simp is_non_redundant; rewrite andTb; apply_andP.
-      apply: exec_preserves_non_existent_label.
-      apply: filtered_queries_hasN_response_name.
-
-    - move=> f α f' args v ty φ qs IH IHqs Hv Hlook; simp is_non_redundant; apply_and3P.
-      apply: exec_preserves_non_existent_label.
-      apply: filtered_queries_hasN_response_name.
-
-    - move=> f α f' args ty φ qs IHqs Hv Hlook; simp is_non_redundant; apply_and3P.
-      apply: exec_preserves_non_existent_label.
-      apply: filtered_queries_hasN_response_name.
-
-    - move=> l f' args ftype f α φ qs IH IHqs Hlook; simp is_non_redundant; apply_and3P.
-      * rewrite all_map; apply/allP => v Hin /=; simp is_non_redundant.
-      * apply: exec_preserves_non_existent_label.
-        apply: filtered_queries_hasN_response_name.
-
-    - move=> l f α φ qs IH Hlook; simp is_non_redundant; rewrite andTb; apply_andP.
-      apply: exec_preserves_non_existent_label.
-      apply: filtered_queries_hasN_response_name.
-
-    - move=> f α v f' args ty l φ qs IH IHqs Hv Hlook; simp is_non_redundant; apply_and3P.
-      apply: exec_preserves_non_existent_label.
-      apply: filtered_queries_hasN_response_name.
-
-    - move=> f α f' args ty l φ qs IHqs Hv Hlook; simp is_non_redundant; apply_and3P.
-      apply: exec_preserves_non_existent_label.
-      apply: filtered_queries_hasN_response_name.
+    all: do ? intros; simp is_non_redundant; apply_and3P;
+      [by rewrite all_map; apply/allP => v Hin /=; simp is_non_redundant| by apply: exec_filtered_queries_asdf].
   Qed.
 
+
+  (*Lemma eval_filter_subseq k (qs : seq (@Query Name Vals)) u :
+    subseq (⟦ filter_queries_with_label k qs ⟧ˢ in u) (⟦ qs ⟧ˢ in u).
+    *)
+    
+ 
+   
+
+
+
+ 
+
+  
+  Theorem grounding_preserves_semantics ty u qs :
+    u.(type) \in get_possible_types s ty ->
+    ⟦ ground s ty qs ⟧ˢ in u = ⟦ qs ⟧ˢ in u.
+  Proof.
+    move: {2}(queries_size _) (leqnn (queries_size qs)) => n.
+    elim: n qs u ty => /= [| n IH] qs u ty.
+    - by rewrite leqn0 => /queries_size_0_nil ->. 
+    - case: qs => //; case=> [f α | l f α | f α φ | l f α φ | t φ] qs /= Hleq Hinpty; simp ground.
+      * case is_object_type => /=; [simp execute_selection_set|].
+        + case lookup_field_in_type => //=; last by apply: IH.
+          by case (u.(fields) _) => /= [[v | vs] |]; rewrite filter_ground_swap IH //;
+             have Hfleq := (filter_queries_with_label_leq_size f qs); ssromega.
+        + simp try_inline_query.
+          case: eqP => /= Heq.
+          simp execute_selection_set.
+          case lookup_field_in_type => //=; last by apply: IH.
+          by case (u.(fields) _) => /= [[v | vs] |]; rewrite filter_ground_swap IH //;
+             have Hfleq := (filter_queries_with_label_leq_size f qs); ssromega.
+
+          admit. (* Inlining field *)
+      * case is_object_type => /=; [simp execute_selection_set|].
+        + case lookup_field_in_type => //=; last by apply: IH.
+          by case (u.(fields) _) => /= [[v | vs] |]; rewrite filter_ground_swap IH //;
+             have Hfleq := (filter_queries_with_label_leq_size l qs); ssromega.
+        + simp try_inline_query.
+          case: eqP => /= Heq.
+          simp execute_selection_set.
+          case lookup_field_in_type => //=; last by apply: IH.
+          by case (u.(fields) _) => /= [[v | vs] |]; rewrite filter_ground_swap IH //;
+             have Hfleq := (filter_queries_with_label_leq_size l qs); ssromega.
+          admit. (* Inlining field *)
+
+      * case Hlook : lookup_field_in_type => [fld|] /=.
+        case Hscope: is_object_type => /=.
+        have Hpty := (get_possible_types_objectE Hscope).
+        have Hinpty2 := Hinpty.
+        rewrite Hpty mem_seq1 /= in Hinpty2; move/eqP in Hinpty2.
+        simp execute_selection_set; rewrite Hinpty2 Hlook /=.
+        case: fld {Hlook} => f' args; case=> rty /=.
+        case ohead => //= [v |].
+        rewrite filter_ground_swap IH //.
+        congr cons; congr pair; congr Object.
+        admit. (* Subqueries with merging *)
+        have Hfleq := (filter_queries_with_label_leq_size f qs); ssromega.
+        rewrite filter_ground_swap IH //; have Hfleq := (filter_queries_with_label_leq_size f qs); ssromega.
+        rewrite filter_ground_swap IH //; last by have Hfleq := (filter_queries_with_label_leq_size f qs); ssromega.
+        
+        congr cons; congr pair; congr Array.
+        apply/eq_in_map => v Hin; congr Object.
+        admit. (* Subqueries with merging *)
+       
+        + (* Inlining *)
+          simp try_inline_query; case: eqP => /= Hpty; [admit |]. (* First one is similar to previous proof, but have to pay attention to abstract scope *)
+          (* lookup f in u should give the same as looking up in ty. 
+             Probably need more info, such as query and graph conformance to show that both 
+             lookups result in the same field definition being fetched *)
+          admit. (* Inline field *)
+
+        + (* Error *)
+          (* Similar to previous one, both lookups should result in the same, if
+             the query and graph conforms. *)
+          admit.
+
+      * admit. (* Copy & Paste *)
+
+      * case Hscope : is_object_type => /=.
+        + case Hfapplies : does_fragment_type_apply => /=.
+          (* fragment type applies *)
+          simp execute_selection_set.
+          have Hpty := (get_possible_types_objectE Hscope).
+          have Hinpty2 := Hinpty.
+          rewrite Hpty mem_seq1 /= in Hinpty2; move/eqP in Hinpty2.
+          rewrite Hinpty2 Hfapplies /= -ground_cat; apply: IH => //; by rewrite queries_size_app; rewrite -/(queries_size φ) in Hleq; ssromega.
+          (* fragment type does not apply *)
+          simp execute_selection_set.
+          have Hinpty2 := Hinpty.
+          have Hpty := (get_possible_types_objectE Hscope).
+          rewrite Hpty mem_seq1 /= in Hinpty2; move/eqP in Hinpty2.
+          rewrite Hinpty2 Hfapplies /=; apply: IH => //; ssromega.
+
+        + case Ht : is_object_type => /=.
+          case Hfapplies : does_fragment_type_apply => /=; simp execute_selection_set; case Huapplies : does_fragment_type_apply => /=.
+          admit. (* Weird case :/ *)
+          apply: IH => //; by ssromega.
+          admit. (* Contradiction : if fragment applies between u & t → u = t → t ∈ possible types of ty → fragment applies between t and ty *)
+          
+          by apply: IH => //; ssromega.
+
+          admit. (* Inlining with intersection of subtypes *)         
+  Admitted.
+
+ 
+  Lemma are_grounded_fields_grounded qs :
+    are_grounded_fields s qs ->
+    are_grounded s qs.
+  Proof.
+    elim: qs => //= q qs IH /and3P [Hfld Hg Hgs]; apply_andP.
+    by rewrite Hfld /=.
+  Qed.
+
+
+
+  
+  Lemma filter_queries_fragments_swap l t (qs : seq (@Query Name Vals)) :
+    filter_queries_with_label l (filter_fragments_with_guard t qs) =
+    filter_fragments_with_guard t (filter_queries_with_label l qs).
+  Admitted.
+
+  Lemma filter_fragments_when_all_fields_is_same t (qs : seq (@Query Name Vals)) :
+    all (fun q => q.(is_field)) qs ->
+    filter_fragments_with_guard t qs = qs.
+  Proof.
+    by funelim (filter_fragments_with_guard t qs) => //= /andP [_ Hflds]; rewrite H //.
+  Qed.
+
+  Lemma filter_fragments_cat t (qs1 qs2 : seq (@Query Name Vals)) :
+    filter_fragments_with_guard t (qs1 ++ qs2) = 
+    filter_fragments_with_guard t qs1 ++ filter_fragments_with_guard t qs2.
+  Admitted.
+
+  Lemma filter_queries_with_label_cat l (qs1 qs2 : seq (@Query Name Vals)):
+    filter_queries_with_label l (qs1 ++ qs2) = filter_queries_with_label l qs1 ++ filter_queries_with_label l qs2.
+  Admitted.
+
+   
+    
+  Lemma asdf q qs1 qs2 u :
+    ⟦ qs1 ⟧ˢ in u = ⟦ qs2 ⟧ˢ in u ->
+    ⟦ q :: qs1 ⟧ˢ in u = ⟦ q :: qs2 ⟧ˢ in u.
+  Proof.
+    by rewrite -2!cat1s; apply: qwe.
+  Qed.
+    
+    
+
+  
+
+ 
+
+  
+  Lemma filter_preserves_grounded_fields k qs :
+    are_grounded_fields s qs ->
+    are_grounded_fields s (filter_queries_with_label k qs).
+  Proof.
+      by funelim (filter_queries_with_label k qs) => //= /and3P [_ Hg Hgs]; do ?apply_and3P; apply: H.
+  Qed.
+
+  Lemma filter_preserves_grounded_inlines k qs :
+    are_grounded_inlines s qs ->
+    are_grounded_inlines s (filter_queries_with_label k qs).
+  Proof.
+    funelim (filter_queries_with_label k qs) => //=; simp is_grounded => /and3P [_ /andP [Hobj Hg] Hgs]; apply_and3P.
+    by apply_andP; apply: filter_preserves_grounded_fields.
+    by apply: H0.
+  Qed.
+  
+  Lemma filter_preserves_grounded k qs :
+    are_grounded s qs ->
+    are_grounded s (filter_queries_with_label k qs).
+  Proof.
+    funelim (filter_queries_with_label k qs) => /=; simp is_field; simp is_grounded => /andP [Hg Hgs].
+    case/andP: Hg; intros; apply_andP.
+      by apply_andP; apply: filter_preserves_grounded_fields.
+      by apply: filter_preserves_grounded_inlines.
+
+      
+      all: do ?[by apply_andP; apply: filter_preserves_grounded_fields].
+      all: do ? [by apply: H; apply: are_grounded_fields_grounded].
+  Qed.
+
+  
+  Lemma filter_preserves_grounded2 ty k qs :
+    are_grounded2 s ty qs ->
+    are_grounded2 s ty (filter_queries_with_label k qs).
+  Proof.
+    funelim (filter_queries_with_label k qs) => //=;
+                                                 rewrite !are_grounded2_clause_2_equation_1;
+                                                 case is_object_type; case: eqP => //= _; case/and3P; intros.
+
+    all: do ? apply_and3P; simp is_grounded2. (* simp is_grounded also works... *)
+    simp is_grounded2 in p0; case/andP: p0; intros.
+    by apply_andP; apply: H.
+  Qed.
+
+  Theorem remove_redundancies_preserves_grounded2_semantics ty u qs :
+    are_grounded2 s ty qs -> 
+    ⟦ remove_redundancies qs ⟧ˢ in u = ⟦ qs ⟧ˢ in u.
+  Proof.
+    funelim (execute_selection_set u qs) => //=.
+
+    - simp remove_redundancies; simp execute_selection_set; rewrite Heq /=. admit.
+    - simp remove_redundancies; simp execute_selection_set; rewrite Heq0 /= Heq /=.
+      rewrite filter_remove_swap filter_filter_absorb; intros. congr cons; apply: (H ty).
+      apply: filter_preserves_grounded2. admit.
+    - simp remove_redundancies; simp execute_selection_set; rewrite Heq0 /= Heq /=.
+      rewrite filter_remove_swap filter_filter_absorb; intros. congr cons; apply: (H ty).
+      apply: filter_preserves_grounded2. admit.
+    - simp remove_redundancies; simp execute_selection_set; rewrite Heq0 /= Heq /=.
+      rewrite filter_remove_swap filter_filter_absorb; intros. congr cons; apply: (H ty).
+      apply: filter_preserves_grounded2. admit.
+
+    - admit.
+    - admit.
+    - admit.
+    - admit.
+
+    - admit.
+    - intros.
+      simp remove_redundancies; simp execute_selection_set; rewrite Heq0 /= Heq /=.
+      congr cons; last first.
+      rewrite filter_remove_swap filter_filter_absorb; apply: (H0 ty); admit.
+      congr pair; congr Array; apply/eq_in_map => v Hin; congr Object.
+      have ->: (find_queries_with_label s s3 v.(type) (remove_redundancies (filter_queries_with_label s3 l))) = [::] by admit.
+      simp merge_selection_sets; rewrite cats0.
+      rewrite -(find_queries_or_fields_is_same_if_all_fields v.(type)).
+      apply: H.
+      admit. (* are subqueries grounded - should be *)
+      admit. (* are all fields in list ? - yes *)
+
+    - intros.
+      simp remove_redundancies; simp execute_selection_set; rewrite Heq1 /= Heq0 /= Heq /=.
+      congr cons; last first.
+      rewrite filter_remove_swap filter_filter_absorb; apply: (H0 ty); admit.
+      congr pair; congr Object.
+      have ->: (find_queries_with_label s s3 n.(type) (remove_redundancies (filter_queries_with_label s3 l))) = [::] by admit.
+      simp merge_selection_sets; rewrite cats0.
+      rewrite -(find_queries_or_fields_is_same_if_all_fields n.(type)).
+      apply: (H f.(return_type)).
+      admit.
+      admit.
+
+    - intros.
+      simp remove_redundancies; simp execute_selection_set; rewrite Heq1 /= Heq0 /= Heq /=; congr cons.
+      rewrite filter_remove_swap filter_filter_absorb; apply: (H ty). admit.
+
+    - admit.
+    - admit.
+    - admit.
+    - admit.
+
+    - intros; simp remove_redundancies; simp execute_selection_set; rewrite Heq /=.
+      admit.
+
+    - intros; simp remove_redundancies; simp execute_selection_set; rewrite Heq /=.
+
+  Abort.
+
+
+  Theorem remove_redundancies_preserves_grounded2_semantics ty u qs :
+    are_grounded2 s ty qs -> 
+    ⟦ remove_redundancies qs ⟧ˢ in u = ⟦ qs ⟧ˢ in u.
+  Proof.
+    funelim (remove_redundancies qs) => //=; rewrite are_grounded2_clause_2_equation_1.
+    - case Hscope : is_object_type; case: eqP => //= Hpty => /and3P [_ _ Hgs].
+      * simp execute_selection_set; case Hlook : lookup_field_in_type => //= [fld|].
+        + by case (u.(fields) _) => /= [[v | vs] |]; congr cons; rewrite filter_remove_swap filter_filter_absorb;
+                                     apply: (H ty) => //; apply: filter_preserves_grounded2.
+          (* lookup = null then semantics is the same *)
+          admit.
+
+      * simp execute_selection_set; case Hlook : lookup_field_in_type => //= [fld|].
+        + by case (u.(fields) _) => /= [[v | vs] |]; congr cons; rewrite filter_remove_swap filter_filter_absorb;
+                                     apply: (H ty) => //; apply: filter_preserves_grounded2.
+          (* lookup = null then semantics is the same *)
+          admit.
+
+    - admit. (* Copy & Paste *)
+
+    - case Hscope : is_object_type; case: eqP => //= Hpty /and3P [_ Hg Hgs]; simp execute_selection_set.
+      * case Hlook : lookup_field_in_type => [fld |] /=.
+        case fld.(return_type) => /= rty.
+
+        + case ohead => [v |] /=.
+          congr cons; last first.
+          rewrite filter_remove_swap filter_filter_absorb; apply: (H0 ty).  H0 //.
+          congr pair; congr Object.
+      
+        
+  Theorem remove_redundancies_preserves_semantics u qs :
+    are_grounded s qs -> 
+    ⟦ remove_redundancies qs ⟧ˢ in u = ⟦ qs ⟧ˢ in u.
+  Proof.
+    funelim (remove_redundancies qs) => //=.
+    - simp is_field => /=; rewrite -/(are_grounded_fields s l) => /andP [Hg Hgflds].
+      simp execute_selection_set; case Hlook : lookup_field_in_type => //= [fld|].
+      * case (u.(fields) _) => /= [[v | vs] |]; congr cons; rewrite filter_remove_swap filter_filter_absorb;
+        by apply: H => //; apply: are_grounded_fields_grounded; apply: filter_preserves_grounded_fields.
+      * rewrite H //; last by apply: filter_preserves_grounded; apply: are_grounded_fields_grounded.
+        (* lookup = null then semantics is the same *)
+        admit.
+        
+    - simp is_field => /=; rewrite -/(are_grounded_fields s l) => /andP [Hg Hgflds].
+      simp execute_selection_set; case Hlook : lookup_field_in_type => //= [fld|].
+     * case (u.(fields) _) => /= [[v | vs] |]; congr cons; rewrite filter_remove_swap filter_filter_absorb;
+        by apply: H => //; apply: are_grounded_fields_grounded; apply: filter_preserves_grounded_fields.
+      * rewrite H //; last by apply: filter_preserves_grounded; apply: are_grounded_fields_grounded.
+        (* lookup = null then semantics is the same *)
+        admit.
+    
+
+    - simp is_field => /=; rewrite -/(are_grounded_fields s l); simp is_grounded => /andP [Hg Hgflds].
+      simp execute_selection_set.
+      case Hlook : lookup_field_in_type => [fld|] //=.
+      * case fld.(return_type) => rty /=; [|congr cons].
+        + case ohead => /= [v |]; congr cons. 
+          congr pair; congr Object.
+          rewrite !find_queries_or_fields_is_same_if_all_fields.
+          have ->: (find_fields_with_response_name Name Vals s3
+                                                   (remove_redundancies (filter_queries_with_label s3 l))) = [::] by admit.
+          simp merge_selection_sets; rewrite cats0 H //.
+          rewrite are_grounded_cat.
+          (* are subqueries grounded ? -> yep, should be simple *)
+          admit.
+            by rewrite are_grounded_fields_E in Hgflds; case/andP: Hgflds.
+            admit. (* remove redundancies preserves fields *)
+            
+            rewrite filter_remove_swap filter_filter_absorb; apply: H0.
+            admit. (* filter preserves grounding *)
+
+            rewrite filter_remove_swap filter_filter_absorb; apply: H0.
+            admit.
+
+        + congr pair; congr Array.
+          apply/eq_in_map => v Hin; congr Object.
+          rewrite !find_queries_or_fields_is_same_if_all_fields.
+          have ->: (find_fields_with_response_name Name Vals s3
+                                                   (remove_redundancies (filter_queries_with_label s3 l))) = [::] by admit.
+          simp merge_selection_sets; rewrite cats0 H //.
+           (* are subqueries grounded ? -> yep, should be simple *)
+          admit.
+          by rewrite are_grounded_fields_E in Hgflds; case/andP: Hgflds.
+          admit. (* remove redundancies preserves fields *)
+            
+          rewrite filter_remove_swap filter_filter_absorb; apply: H0.
+          admit.
+          admit.
+
+    - simp is_field => /=; rewrite -/(are_grounded_fields s l); simp is_grounded => /andP [Hg Hgflds].
+      simp execute_selection_set.
+      case Hlook : lookup_field_in_type => [fld|] //=.
+      * case fld.(return_type) => rty /=; [|congr cons].
+        + case ohead => /= [v |]; congr cons. 
+          congr pair; congr Object.
+          rewrite !find_queries_or_fields_is_same_if_all_fields.
+          have ->: (find_fields_with_response_name Name Vals s4
+                                                   (remove_redundancies (filter_queries_with_label s4 l))) = [::] by admit.
+          simp merge_selection_sets; rewrite cats0 H //.
+          (* are subqueries grounded ? -> yep, should be simple *)
+          admit.
+            by rewrite are_grounded_fields_E in Hgflds; case/andP: Hgflds.
+            admit. (* remove redundancies preserves fields *)
+            
+            rewrite filter_remove_swap filter_filter_absorb; apply: H0.
+            admit. (* filter preserves grounding *)
+
+            rewrite filter_remove_swap filter_filter_absorb; apply: H0.
+            admit.
+
+        + congr pair; congr Array.
+          apply/eq_in_map => v Hin; congr Object.
+          rewrite !find_queries_or_fields_is_same_if_all_fields.
+          have ->: (find_fields_with_response_name Name Vals s4
+                                                   (remove_redundancies (filter_queries_with_label s4 l))) = [::] by admit.
+          simp merge_selection_sets; rewrite cats0 H //.
+           (* are subqueries grounded ? -> yep, should be simple *)
+          admit.
+          by rewrite are_grounded_fields_E in Hgflds; case/andP: Hgflds.
+          admit. (* remove redundancies preserves fields *)
+            
+          rewrite filter_remove_swap filter_filter_absorb; apply: H0.
+          admit.
+          admit.
+
+    - simp is_field; rewrite -/(are_grounded_inlines s l); simp is_grounded => /andP [/andP [Htobj Hgflds] Hginls].
+      simp execute_selection_set.
+      case Hfapplies : does_fragment_type_apply => //=.
+      admit.
+
+      (* removing invalid fragments preserves semantics *)
+      rewrite H0.
+      apply: filtering_invalid_fragments_preserves_semantics => //.
+      admit.
+
+
+
+
+
+
+          
+  
+    
+  Lemma fragment_applies_for_node u : does_fragment_type_apply s u.(type) u.(type). Admitted.
+  
+  Lemma normalize_preserves_semantics ty u qs :
+    ⟦ normalize s ty qs in u ⟧ˢ = ⟦ qs in u ⟧ˢ.
+  Proof.
+    rewrite /normalize /=.
+    rewrite (remove_redundancies_preserves_semantics u (ground s ty qs)).
+    by rewrite grounding_preserves_semantics.
+  Qed.
+  
+
+
+  
   Reserved Notation "⦃ queries 'in' u ⦄" (at level 50).
   
    Equations? execute_selection_set2 u (queries : seq (@Query Name Vals)) :
@@ -309,9 +1881,10 @@ Section QuerySemantic.
   Proof.
     elim: qs1  => //= hd tl IH.
     case: hd => //=; intros; simp filter_queries_with_label; do ?[by case: eqP => //= Heq; rewrite IH].
-      by rewrite IH.
+    by rewrite IH.
   Qed.
-    
+
+  (*
   Lemma normalize_filter_swap label ty qs :
     is_object_type s ty ->
     filter_queries_with_label label (normalize__φ s ty qs) = normalize__φ s ty (filter_queries_with_label label qs).
@@ -347,7 +1920,7 @@ Section QuerySemantic.
     lookup_field_in_type s ty f = Some fld ->
     lookup_field_type s ty f = Some (fld.(return_type)).
   Admitted.
-
+*)
    
   Transparent is_field is_inline_fragment qresponse_name qsubqueries.
 
@@ -362,6 +1935,7 @@ Section QuerySemantic.
   Proof.
     funelim (are_similar q1 q2) => //=.
   Qed.
+
   
   Lemma filter_not_similar_preserves_list (q : @Query Name Vals) qs (Hfield : q.(is_field)) :
     all (fun q' => ~~are_similar q' q) qs ->
@@ -385,7 +1959,35 @@ Section QuerySemantic.
                   all (is_in_normal_form s) qs ->
                   are_in_normal_form s qs.
   Admitted.
+
+
+
+ 
+
+    
+  Lemma all_invalid_fragments_exec u φ qs :
+    all (fun q => q.(is_inline_fragment)) qs ->
+    are_in_normal_form s qs ->
+    all (fun q => ~~are_similar q (InlineFragment u.(type) φ)) qs ->
+    ⟦ φ ++ qs in u ⟧ˢ = ⟦ φ in u ⟧ˢ. 
+  Proof.
+    move: {2}(queries_size _) (leqnn (queries_size φ)) => n.
+    elim: n φ qs => [| n IH] φ qs Hleq.
+    - admit.
+    -admit.
+  Admitted.
+
+
+
   
+  Lemma execute_selection_set_on_nrgt u qs :
+    are_non_redundant qs ->
+    are_in_normal_form s qs ->
+    ⟦ qs in u ⟧ˢ = flatten [seq ⟦ [:: q] in u ⟧ˢ | q <- qs].
+  Proof.
+    Abort.
+    
+        
   Theorem execs_on_nrgtnf_are_equivalent u φ :
     are_in_normal_form s φ ->
     are_non_redundant φ ->
@@ -393,62 +1995,72 @@ Section QuerySemantic.
   Proof.
     move: {2}(queries_size _) (leqnn (queries_size φ)) => n.
     elim: n φ u => [| n IH] φ u.
-    - admit.
+    - by rewrite leqn0 => /queries_size_0_nil ->. 
     - case: φ => //=; case=> /= [f α | l f α | f α φ | l f α φ | t φ] qs Hleq.
-      * rewrite /are_in_normal_form /= orbF; simp is_in_normal_form; rewrite andTb => /andP [Hflds Hnf].
+      * simp are_in_normal_form => /andP [Hflds Hnf].
         simp are_non_redundant; rewrite andTb => /=-/andP [Hneq Hnr].
         simp execute_selection_set; simp execute_selection_set2.
         case: (u.(fields) _) => //=; [case=> // v|];
                                  rewrite (filter_not_similar_preserves_list (SingleField f α)) // IH //; by apply: asdf.
       
-      * rewrite /are_in_normal_form /= orbF; simp is_in_normal_form; rewrite andTb => /andP [Hflds Hnf].
+      * simp are_in_normal_form => /andP [Hflds Hnf].
         simp are_non_redundant; rewrite andTb => /=-/andP [Hneq Hnr].
         simp execute_selection_set; simp execute_selection_set2.
         case: (u.(fields) _) => //=; [case=> // v|];
                                  rewrite (filter_not_similar_preserves_list (LabeledField l f α)) // IH //; by apply: asdf.
 
         
-      * rewrite /are_in_normal_form /= orbF; simp is_in_normal_form => /and3P [Hfld /andP [Hty Hnf] Hnfs].
+      * simp are_in_normal_form => /and3P [Hnf Hfields Hnfs].
         simp are_non_redundant => /= /and3P [Hsim Hnr Hnrs]. 
         simp execute_selection_set; simp execute_selection_set2.
         case Hlook : lookup_field_in_type => [fld|] //=; last rewrite (filter_not_similar_preserves_list (NestedField f α φ)) //.
         case: fld Hlook => f' args; case=> ty Hlook /=. 
         + case ohead => //= [v|]; rewrite (filter_not_similar_preserves_list (NestedField f α φ)) //.
           rewrite (find_not_similar_is_nil v.(type) (NestedField f α φ)) //; simp merge_selection_sets.
-          rewrite cats0 !IH //; admit.
-          rewrite IH //; admit.
-
+          by rewrite cats0 !IH //; rewrite -/(queries_size φ) in Hleq; ssromega.
+          by rewrite IH //; ssromega.
+          
         + rewrite (filter_not_similar_preserves_list (NestedField f α φ)) //. 
-          congr cons; [| apply: IH; admit].
-          congr pair; congr Array. apply/eq_in_map => v Hin.
+          congr cons; last by apply: IH => //; ssromega.
+          congr pair; congr Array.
+          apply/eq_in_map => v Hin.
           rewrite (find_not_similar_is_nil v.(type) (NestedField f α φ)) //; simp merge_selection_sets.
-          rewrite cats0 IH //; admit.
-        + rewrite IH //; admit.
-
+            by rewrite cats0 !IH //; rewrite -/(queries_size φ) in Hleq; ssromega.
+        + by rewrite IH //; ssromega.
              
-      * rewrite /are_in_normal_form /= orbF; simp is_in_normal_form => /and3P [Hfld /andP [Hty Hnf] Hnfs].
+      * simp are_in_normal_form => /and3P [Hnf Hfields Hnfs].
         simp are_non_redundant => /= /and3P [Hsim Hnr Hnrs]. 
         simp execute_selection_set; simp execute_selection_set2.
         case Hlook : lookup_field_in_type => [fld|] //=; last rewrite (filter_not_similar_preserves_list (NestedLabeledField l f α φ)) //.
         case: fld Hlook => f' args; case=> ty Hlook /=. 
         + case ohead => //= [v|]; rewrite (filter_not_similar_preserves_list (NestedLabeledField l f α φ)) //.
           rewrite (find_not_similar_is_nil v.(type) (NestedLabeledField l f α φ)) //; simp merge_selection_sets.
-          rewrite cats0 !IH //; admit.
-          rewrite IH //; admit.
-
+            by rewrite cats0 !IH //; rewrite -/(queries_size φ) in Hleq; ssromega.
+          by rewrite IH //; ssromega.
+         
         + rewrite (filter_not_similar_preserves_list (NestedLabeledField l f α φ)) //. 
-          congr cons; [| apply: IH; admit].
-          congr pair; congr Array. apply/eq_in_map => v Hin.
+          congr cons; last by apply: IH => //; ssromega.
+          congr pair; congr Array.
+          apply/eq_in_map => v Hin.
           rewrite (find_not_similar_is_nil v.(type) (NestedLabeledField l f α φ)) //; simp merge_selection_sets.
-          rewrite cats0 IH //; admit.
-        + rewrite IH //; admit.
+            by rewrite cats0 !IH //; rewrite -/(queries_size φ) in Hleq; ssromega.
+        + by rewrite IH //; ssromega. 
 
-
-      * rewrite /are_in_normal_form /=; simp is_in_normal_form => Hnf.
+      * simp are_in_normal_form => /and5P [Hobj Hflds Hnf Hinl Hnfs].
         simp are_non_redundant => /= /and3P [Hsim Hnr Hnrs].
         simp execute_selection_set; simp execute_selection_set2.
-        case: does_fragment_type_apply => //=; apply: IH.
-  Admitted.
+        case Hfrag: does_fragment_type_apply => //=; last by apply: IH => //; ssromega.
+        rewrite execute_selection_set2_cat.
+        rewrite (all_invalid_fragments_eval u φ qs) // ?cats0; last first.
+        rewrite /does_fragment_type_apply Hobj in Hfrag.
+          by move/eqP in Hfrag; rewrite Hfrag.        
+        
+          
+        rewrite all_invalid_fragments_exec //; [apply: IH => //; rewrite -/(queries_size φ) in Hleq; ssromega|].
+        rewrite /does_fragment_type_apply Hobj in Hfrag.
+          by move/eqP in Hfrag; rewrite Hfrag.
+  Qed.
+  
 
         
   
